<?xml version="1.0" encoding="ISO-8859-1" standalone="yes"?>
<!--
  Data HUb Service (DHuS) - For Space data distribution.
  Copyright (C) 2021 European Space Agency (ESA)
  Copyright (C) 2021 GAEL Systems
  Copyright (C) 2021 Serco Spa

  This file is part of DHuS software sources.

  This program is free software: you can redistribute it and/or modify
  it under the terms of the GNU Affero General Public License as
  published by the Free Software Foundation, either version 3 of the
  License, or (at your option) any later version.

  This program is distributed in the hope that it will be useful,
  but WITHOUT ANY WARRANTY; without even the implied warranty of
  MERCHANTABILITY or FITNESS FOR A PARTICULAR PURPOSE. See the
  GNU Affero General Public License for more details.

  You should have received a copy of the GNU Affero General Public License
  along with this program. If not, see <http://www.gnu.org/licenses/>.

-->

<!DOCTYPE rdf:RDF [
   <!ENTITY rdf  "http://www.w3.org/1999/02/22-rdf-syntax-ns#">
   <!ENTITY rdfs "http://www.w3.org/2000/01/rdf-schema#">
   <!ENTITY owl  "http://www.w3.org/2002/07/owl#">
   <!ENTITY s3   "http://www.esa.int/s3#">
   <!ENTITY drb  "http://www.gael.fr/drb#">
   <!ENTITY jpeg "http://www.gael.fr/drb/jpeg#">
]>
<rdf:RDF xmlns:owl="&owl;"
         xmlns:rdf="&rdf;"
         xmlns:rdfs="&rdfs;"
         xmlns:drb="&drb;"
         xmlns:jpeg="&jpeg;"
         xmlns:s3="&s3;"
         xml:base="&s3;">

   <owl:Ontology rdf:about="&s3;">
      <rdfs:label xml:lang="en">Sentinel-3 - Auxiliary products Ontology</rdfs:label>
   </owl:Ontology>

   <!-- ================================================================== -->
   <!-- Sentinel-3 Auxiliary EOF abstract class                            -->
   <!-- WARN this class is not a subclass of 'Sentinel-3 Product'          -->
   <!--                                   or 'Sentinel-3 Auxiliary Product'-->
   <!-- ================================================================== -->

   <!-- ================================================ -->
   <!-- Sentinel-3 POD Abstract class                    -->
   <!-- ================================================ -->

   <owl:Class rdf:about="&s3;auxiliaryEofPod">
      <rdfs:label xml:lang="en">Sentinel-3 EOF Precise Orbit Determination (POD) Auxiliary Product</rdfs:label>
      <rdfs:comment xml:lang="en">
         Generic class for POD products.
      </rdfs:comment>
      <rdfs:subClassOf rdf:resource="&drb;item"/>
      <drb:signature rdf:parseType="Resource">
         <drb:nameMatch>S3._(...._AUX_(RESORB|PREORB|MOEORB|POEORB|PRCPTF)_|SR___ROE_AX).*EOF</drb:nameMatch>
      </drb:signature>
      <drb:implementationIdentifier>xml</drb:implementationIdentifier>
   </owl:Class>

   <!-- ================================================ -->
   <!-- Sentinel-3 AUX_POEORB                            -->
   <!-- ================================================ -->

   <!-- Example S3B_OPER_AUX_POEORB_POD__20181101T081009_V20181006T215942_20181007T235942_DGNS.EOF -->
   <owl:Class rdf:about="&s3;auxiliaryEofPodPoeorb">
      <rdfs:label xml:lang="en">Sentinel-3 EOF Precise Orbit Ephemerides Orbit File Auxiliary Product</rdfs:label>
      <rdfs:comment xml:lang="en">
         This file contains the Precise Orbit Ephemerides (POE) Restituted
         Orbit State Vectors (OSV) based on the orbit determination performed
         by the POD Service. The OSVs refer to the CoG of the satellite and
         are expressed in Earth-fixed Coordinate Frame.
      </rdfs:comment>
      <rdfs:subClassOf rdf:resource="&s3;auxiliaryEofPod"/>
      <drb:signature rdf:parseType="Resource">
         <drb:nameMatch>S3(A|B)_...._AUX_POEORB_.*</drb:nameMatch>
      </drb:signature>
   </owl:Class>

   <!-- ================================================ -->
   <!-- Sentinel-3 AUX_MOEORB                            -->
   <!-- ================================================ -->

   <!-- Example S3A_OPER_AUX_MOEORB_POD__20181113T081223_V20181111T215942_20181112T235942_DGNS.EOF -->
   <owl:Class rdf:about="&s3;auxiliaryEofPodMoeorb">
      <rdfs:label xml:lang="en">Sentinel-3 EOF Medium Orbit Ephemerides Auxiliary Product</rdfs:label>
      <rdfs:comment xml:lang="en">
         This file contains the Medium Orbit Ephemerides (MOE), corresponding
         to the Preliminary Restituted Orbit State Vectors (OSV) based on the
         orbit determination performed by the POD Service Centre. The Orbit
         State Vectors refer to the CoG of the satellite and are expressed in
         Earth-fixed Coordinate Frame. The file also contains quality indicator
         parameters.
      </rdfs:comment>
      <rdfs:subClassOf rdf:resource="&s3;auxiliaryEofPod"/>
      <drb:signature rdf:parseType="Resource">
         <drb:nameMatch>S3(A|B)_...._AUX_MOEORB_.*</drb:nameMatch>
      </drb:signature>
   </owl:Class>

   <!-- ================================================ -->
   <!-- Sentinel-3 AUX_PRCPTF                            -->
   <!-- ================================================ -->

   <!-- Example S3A_OPER_AUX_PRCPTF_POD__20181113T071050_V20181018T215942_20181019T235942.EOF -->
   <owl:Class rdf:about="&s3;auxiliaryEofPodPrcptf">
      <rdfs:label xml:lang="en">Sentinel-3 EOF Precise Platform Data Auxiliary Product</rdfs:label>
      <rdfs:comment xml:lang="en">
         Two files are foreseen to be generated with different timeliness:
         1. Preliminary Platform file (AUX_PRLPTF);
         2. Precise Platform file (AUX_PRCPTF).
         Both files contain information on:
         * the nadir projection of the distance between the altimeter antenna
         centre of phase and the satellite centre of gravity (m);
         * the platform derived off nadir angles pitch, roll and yaw (degrees);
         The files also contain quality indicator parameters.
      </rdfs:comment>
      <rdfs:subClassOf rdf:resource="&s3;auxiliaryEofPod"/>
      <drb:signature rdf:parseType="Resource">
         <drb:nameMatch>S3(A|B)_...._AUX_PRCPTF_.*</drb:nameMatch>
      </drb:signature>
   </owl:Class>

   <!-- ================================================ -->
   <!-- Sentinel-3 SR___ROE_AX                           -->
   <!-- ================================================ -->

   <!-- Example S3A_SR___ROE_AX_20181113T020209_20181113T034619_20181113T041228___________________POD_O_NR____.EOF -->
   <owl:Class rdf:about="&s3;auxiliaryEofRoe">
      <rdfs:label xml:lang="en">Sentinel-3 EOF NRT Restituted Orbit State Vectors Auxiliary Product</rdfs:label>
      <rdfs:comment xml:lang="en">
         This file contains the NRT Restituted Orbit State Vectors (OSV) based
         on the orbit determination performed by the S-3 NRT POD IPF Facility.
         The Orbit State Vectors refer to the CoG of the satellite and are
         expressed in Earth-fixed Coordinate Frame.
      </rdfs:comment>
      <rdfs:subClassOf rdf:resource="&s3;auxiliaryEofPod"/>
      <drb:signature rdf:parseType="Resource">
         <drb:nameMatch>S3(A|B)_SR___ROE_AX_.*</drb:nameMatch>
      </drb:signature>
   </owl:Class>

   <!-- ================================================================== -->
   <!-- Sentinel-3 Auxiliary SALP -> PDGS INTERFACE                        -->
   <!-- WARN this class is not a subclass of 'Sentinel-3 Product'          -->
   <!--                                   or 'Sentinel-3 Auxiliary Product'-->
   <!-- ================================================================== -->

   <!-- ================================================ -->
   <!-- Sentinel-3 SALP -> PDGS INTERFACE                -->
   <!-- ================================================ -->

   <!-- Examples
        S3A_SR___MDO_AX_20220705T215523_20220707T002323_20220707T080706___________________CNE_O_ST____.TGZ
        S3A_SR___POE_AX_20220607T215523_20220609T002323_20220629T095739___________________CNE_O_NT____.TGZ
        S3B_SR___MDO_AX_20220705T215523_20220707T002323_20220707T082451___________________CNE_O_ST____.TGZ
        S3B_SR___POE_AX_20220607T215523_20220609T002323_20220629T112236___________________CNE_O_NT____.TGZ -->

   <owl:Class rdf:about="&s3;auxiliarySALP-PDGS">
      <rdfs:label xml:lang="en">Sentinel-3 SALP / PDGS INTERFACE Auxiliary TGZ Product</rdfs:label>
      <rdfs:comment xml:lang="en">
         Sentinel-3 SALP / PDGS INTERFACE Auxiliary TGZ Product.
      </rdfs:comment>
      <rdfs:subClassOf rdf:resource="&drb;tgz"/>
      <drb:signature rdf:parseType="Resource">
         <drb:nameMatch>S3(A|B)_SR___(MDO|POE)_AX.*</drb:nameMatch>
      </drb:signature>
   </owl:Class>

   <owl:Class rdf:about="&s3;auxiliarySALP-PDGSEOFFile">
      <rdfs:label xml:lang="en">Sentinel-3 SALP / PDGS INTERFACE EOF File</rdfs:label>
      <rdfs:comment xml:lang="en">
         Sentinel-3 SALP / PDGS INTERFACE EOF File.
      </rdfs:comment>
      <rdfs:subClassOf rdf:resource="&drb;item"/>
      <drb:signature rdf:parseType="Resource">
         <drb:nameMatch>S3(A|B)_SR___(MDO|POE)_AX.*EOF</drb:nameMatch>
      </drb:signature>
      <drb:implementationIdentifier>xml</drb:implementationIdentifier>
   </owl:Class>

   <owl:Class rdf:about="&s3;auxiliarySALP-PDGSXMLFile">
      <rdfs:label xml:lang="en">Sentinel-3 SALP / PDGS INTERFACE XML File</rdfs:label>
      <rdfs:comment xml:lang="en">
         Sentinel-3 SALP / PDGS INTERFACE XML File.
      </rdfs:comment>
      <rdfs:subClassOf rdf:resource="&drb;xml"/>
      <drb:signature rdf:parseType="Resource">
         <drb:nameMatch>S3(A|B)_SR___(MDO|POE)_AX.*XML</drb:nameMatch>
      </drb:signature>
   </owl:Class>

   <!-- ================================================ -->
   <!-- Sentinel-3 SALP -> SR___MDO_AX                   -->
   <!-- ================================================ -->

   <!-- Examples
        S3A_SR___MDO_AX_20220705T215523_20220707T002323_20220707T080706___________________CNE_O_ST____.TGZ
        S3B_SR___MDO_AX_20220705T215523_20220707T002323_20220707T082451___________________CNE_O_ST____.TGZ -->

   <owl:Class rdf:about="&s3;auxiliarySALP-PDGS-Mdo">
      <rdfs:label xml:lang="en">Sentinel-3 SALP / PDGS INTERFACE - SRAL MDO Auxiliary Product</rdfs:label>
      <rdfs:comment xml:lang="en">
         Sentinel-3 SALP / PDGS INTERFACE SRAL MDO Auxiliary Product.
      </rdfs:comment>
      <rdfs:subClassOf rdf:resource="&s3;auxiliarySALP-PDGS"/>
      <drb:signature rdf:parseType="Resource">
         <drb:nameMatch>S.._SR___MDO.*</drb:nameMatch>
      </drb:signature>
   </owl:Class>

   <!-- ================================================ -->
   <!-- Sentinel-3 SALP -> SR___POE_AX                   -->
   <!-- ================================================ -->

   <!-- Examples
        S3A_SR___POE_AX_20220607T215523_20220609T002323_20220629T095739___________________CNE_O_NT____.TGZ
        S3B_SR___POE_AX_20220607T215523_20220609T002323_20220629T112236___________________CNE_O_NT____.TGZ -->

   <owl:Class rdf:about="&s3;auxiliarySALP-PDGS-Poe">
      <rdfs:label xml:lang="en">Sentinel-3 SALP / PDGS INTERFACE - SRAL POE Auxiliary Product</rdfs:label>
      <rdfs:comment xml:lang="en">
         Sentinel-3 SALP / PDGS INTERFACE SRAL POE Auxiliary Product.
      </rdfs:comment>
      <rdfs:subClassOf rdf:resource="&s3;auxiliarySALP-PDGS"/>
      <drb:signature rdf:parseType="Resource">
         <drb:nameMatch>S.._SR___POE.*</drb:nameMatch>
      </drb:signature>
   </owl:Class>

</rdf:RDF>
